prove swap_ok and stackswap_ok

bedrock2/src/bedrock2Examples/swap.v
@@ -1,17 +1,21 @@
 Require Import bedrock2.NotationsCustomEntry coqutil.Macros.WithBaseName.
-
+Require Import coqutil.Tactics.fwd.
+Require Import Lia.
 Import Syntax BinInt String List.ListNotations.
 Local Open Scope string_scope. Local Open Scope Z_scope. Local Open Scope list_scope.
 
 Definition swap := func! (a, b) {
-  t = load(b);
-  store(b, load(a));
-  store(a, t)
+  load1(t, b);
+  load1(x0, a);
+  store1(b, x0);
+  store1(a, t)
 }.
 
 Definition bad_swap := func! (a, b) {
-  store(b, load(a));
-  store(a, load(b))
+  load1(x0, a);
+  store1(b, x0);
+  load1(x1, b);
+  store1(a, x1)
 }.
 
 Definition swap_swap := func! (a, b) {
@@ -19,63 +23,380 @@ Definition swap_swap := func! (a, b) {
   swap(a, b)
 }.
 
-Require Import bedrock2.LeakageWeakestPrecondition.
-Require Import bedrock2.Semantics bedrock2.LeakageSemantics bedrock2.FE310CSemantics.
+Require Import bedrock2.WeakestPrecondition.
+Require Import bedrock2.Semantics.
 Require Import coqutil.Map.Interface bedrock2.Map.Separation bedrock2.Map.SeparationLogic.
 
-Require bedrock2.LeakageWeakestPreconditionProperties.
+Require bedrock2.WeakestPreconditionProperties.
 From coqutil.Tactics Require Import Tactics letexists eabstract.
-Require Import bedrock2.LeakageProgramLogic bedrock2.Scalars.
+Require Import bedrock2.ProgramLogic bedrock2.Scalars.
 Require Import coqutil.Word.Interface.
 Require Import coqutil.Tactics.rdelta.
+Require Import bedrock2.MemList.
+Check Scalars.load_one_of_sep.
+Require Import coqutil.Map.Properties.
+Require Import coqutil.Word.Bitwidth.
 
 Section WithParameters.
-  Context {word: word.word 32} {mem: map.map word Byte.byte}.
-  Context {word_ok: word.ok word} {mem_ok: map.ok mem}.
-  Context {pick_sp: PickSp}.
-
+  Context {BW: Bitwidth 32} {word: word.word 32} {mem: map.map word Byte.byte} {listmem: map.map (word * nat) Byte.byte} {locals: map.map String.string word}.
+  Context {word_ok: word.ok word} {locals_ok: map.ok locals} {mem_ok: map.ok mem} {listmem_ok: map.ok listmem}.
+  Context {ext_spec: ExtSpec} {ext_spec_ok: ext_spec.ok ext_spec}.
+  Locate "=*".
   Instance spec_of_swap : spec_of "swap" :=
-    fnspec! exists f, "swap" a_addr b_addr / a b R,
-    { requires k t m := m =* scalar a_addr a * scalar b_addr b * R;
-      ensures K T M :=  M =* scalar a_addr b * scalar b_addr a * R /\ T = t /\
-                          K = f a_addr b_addr ++ k }.
+    fnspec! "swap" a_addr b_addr / a b R,
+    { requires t m := m =* ptsto a_addr a * ptsto b_addr b * R;
+      ensures T M :=  M =* ptsto a_addr b * ptsto b_addr a * R /\ T = t }.
 
-  Lemma swap_ok : program_logic_goal_for_function! swap.
-  Proof. repeat straightline. intuition eauto. align_trace. Qed.
+  Check cmd. Print cmd.load.
+  Check load_one_of_sep. Check dexpr.
+  Lemma load_one_of_sep_memlist t m l addr value R x ea e  :
+    m =* ptsto addr value * R ->
+    dexpr l ea addr ->
+    cmd e (cmd.load x access_size.one ea) t m l
+      (fun t' m' l' => t' = t /\ m' = m /\ l' = map.put l x (of_bytes [value])).
+  Proof.
+    intros Hm Ha. cbn [cmd cmd_body]. exists addr. split; [assumption|].
+    exists [value]. destruct Hm as (mLoad&mSmall&Hsplit&Hload&Hsmall).
+    exists mLoad, mSmall. split; [reflexivity|]. split.
+    { simpl. exists mLoad, map.empty. ssplit.
+      - apply map.split_empty_r. reflexivity.
+      - assumption.
+      - cbv [emp]. auto. }
+    auto.
+  Qed. Check cmd.store.
 
-  Instance spec_of_bad_swap : spec_of "bad_swap" :=
-    fnspec! exists f, "bad_swap" a_addr b_addr / a b R,
-    { requires k t m := m =* scalar a_addr a * scalar b_addr b * R;
-      ensures K T M :=  M =* scalar a_addr b * scalar b_addr a * R /\ T = t /\
-                          K = f a_addr b_addr ++ k }.
+  Lemma store_one_of_sep_memlist t m l addr val0 val R ea ev e :
+    m =* ptsto addr val0 * R ->
+    dexpr l ea addr ->
+    dexpr l ev val ->
+    cmd e (cmd.store access_size.one ea ev) t m l
+      (fun t' m' l' =>
+         t' = t /\ m' =* ptsto addr (Byte.byte.of_Z (word.unsigned val)) * R /\ l' = l).
+  Proof.
+    intros Hm Ha Hv. cbn [cmd cmd_body]. exists addr. split; [assumption|].
+    exists val. split; [assumption|]. destruct Hm as (mStore&mSmall&Hsplit&Hstore&Hsmall).
+    exists mStore. assert (Hstore' := Hstore). destruct Hstore as [n Hstore].
+    exists (map.put map.empty (addr, n) (Byte.byte.of_Z (word.unsigned val))).
+    exists mSmall. eexists. ssplit.
+    - cbv [anybytes']. exists [val0]. split; [reflexivity|]. exists mStore, map.empty. ssplit.
+      + apply map.split_empty_r. reflexivity.
+      + assumption.
+      + simpl. cbv [emp]. auto.
+    - simpl. eexists. exists map.empty. ssplit.
+      + apply map.split_empty_r. reflexivity.
+      + exists n. reflexivity.
+      + cbv [emp]. auto.
+    - assumption.
+    - cbv [map.split]. split; [reflexivity|]. destruct Hsplit as [_ Hdisj].
+      eapply map.sub_domain_disjoint. 1: eassumption. subst. repeat intro.
+      rewrite map.get_put_dec in H. destruct_one_match_hyp.
+      + eexists. rewrite map.get_put_same. reflexivity.
+      + Search map.get map.empty. rewrite map.get_empty in H. congruence.
+    - reflexivity.
+    - eexists. eexists. ssplit.
+      + split. 1: reflexivity. destruct Hsplit as [_ Hdisj].
+      eapply map.sub_domain_disjoint. 1: eassumption. subst. repeat intro.
+      rewrite map.get_put_dec in H. destruct_one_match_hyp.
+      -- eexists. rewrite map.get_put_same. reflexivity.
+      -- Search map.get map.empty. rewrite map.get_empty in H. congruence.
+      + exists n. reflexivity.
+      + assumption.
+    - reflexivity.
+  Qed.
   
-  Lemma bad_swap_ok : program_logic_goal_for_function! bad_swap.
-  Proof. repeat straightline. intuition eauto; align_trace. Abort.
+  Lemma cmd_seq e s1 s2 t m l post :
+    cmd e (cmd.seq s1 s2) t m l post =
+      cmd e s1 t m l
+        (fun (t0 : trace) (m0 : listmem) (l0 : locals) => cmd e s2 t0 m0 l0 post).
+  Proof. reflexivity. Qed.
 
-  Definition spec_of_swap_same : spec_of "swap" :=
-    fnspec! exists f, "swap" a_addr b_addr / a R,
-    { requires k t m := m =* scalar a_addr a * R /\ b_addr = a_addr;
-      ensures K T M :=  M =* scalar a_addr a * R /\ T = t /\ K = f a_addr ++ k }.
+  Lemma sep_assoc (m : listmem) R1 R2 R3 :
+    m =* R1 * R2 * R3 <-> m =* R1 * (R2 * R3).
+  Proof.
+    split; intros H.
+    - cbv [sep map.split] in *. fwd. exists mp0, (map.putmany mq0 mq).
+      apply map.disjoint_putmany_l in Hp0p1. fwd. ssplit; eauto.
+      + symmetry. apply map.putmany_assoc.
+      + Search (map.disjoint _ (map.putmany _ _)). 
+        apply map.disjoint_putmany_r. eauto.
+      + eauto 10.
+    - cbv [sep map.split] in *. fwd. exists (map.putmany mp mp0), mq0.
+      apply map.disjoint_putmany_r in Hp0p1. fwd. ssplit; eauto.
+      + apply map.putmany_assoc.
+      + Search (map.disjoint _ (map.putmany _ _)). 
+        apply map.disjoint_putmany_l. eauto.
+      + eauto 10.
+  Qed.
 
-  Lemma swap_same_ok :
-    let spec_of_swap := spec_of_swap_same in
-    program_logic_goal_for_function! swap.
-  Proof. repeat straightline. intuition eauto. align_trace. Qed.
+  Lemma sep_comm (m : listmem) R1 R2 :
+    m =* R1 * R2 <-> m =* R2 * R1.
+  Proof.
+    split; intros H; cbv [sep map.split] in *; fwd.
+    - exists mq, mp. intuition auto.  2: apply map.disjoint_comm; assumption.
+      Search map.putmany. apply map.putmany_comm. assumption.
+    - exists mq, mp. intuition auto. 2: apply map.disjoint_comm; assumption.
+      apply map.putmany_comm. assumption.
+  Qed.
 
-  Instance spec_of_swap_swap : spec_of "swap_swap" :=
-    fnspec! "swap_swap" a_addr b_addr / a b R,
-    { requires k t m := m =* scalar a_addr a * scalar b_addr b * R;
-      ensures K T M :=  M =* scalar a_addr a * scalar b_addr b * R /\ T = t }.
+  Lemma idk (m : listmem) R1 R1' R2 :
+    (forall m, m =* R1 <-> m =* R1') ->
+    m =* R1 * R2 <-> m =* R1' * R2.
+  Proof.
+    intros H. split; intros H'; cbv [sep] in *; fwd.
+    - exists mp, mq. ssplit; try assumption. apply H. assumption.
+    - exists mp, mq. ssplit; try assumption. apply H. assumption.
+  Qed.
 
-  Lemma swap_swap_ok : program_logic_goal_for_function! swap_swap.
-  Proof. repeat (straightline || straightline_call); eauto. Qed.
+  Lemma byte_to_word_to_byte b :
+    Byte.byte.of_Z (word.unsigned (word := word) (of_bytes [b])) = b.
+  Proof.
+    cbv [of_bytes]. cbv [LittleEndianList.le_combine].
+    rewrite word.unsigned_of_Z. simpl. Search (Z.lor _ 0). rewrite Z.lor_0_r.
+    Search Byte.byte.unsigned. rewrite wrap_byte_unsigned. Search Byte.byte.unsigned.
+    rewrite Byte.byte.of_Z_unsigned. reflexivity.
+  Qed.
+    
+  Lemma swap_ok : program_logic_goal_for_function! swap.
+  Proof.
+    (*first load*)
+    repeat straightline. subst c1. rewrite cmd_seq.
+    Print seprewrite_in. Print seprewrite0_in.
+    erewrite idk in H.
+    2: { intros. instantiate (1 := (ptsto b_addr b * ptsto a_addr a)%sep). apply sep_comm. }
+    rewrite sep_assoc in H.
+    eapply WeakestPreconditionProperties.Proper_cmd.
+    2: { eapply load_one_of_sep_memlist. 1: eassumption.
+         cbv [dexpr expr expr_body get]. eexists. subst l.
+         rewrite map.get_put_same. auto. }
+    (*second load*)
+    cbv [Morphisms.pointwise_relation Basics.impl]. intros. fwd. subst c0.
+    rewrite cmd_seq.
+    rewrite <- sep_assoc in H. erewrite idk in H.
+    2: { intros. instantiate (1 := (ptsto a_addr a * ptsto b_addr b)%sep).
+         apply sep_comm. }
+    rewrite sep_assoc in H.
+    eapply WeakestPreconditionProperties.Proper_cmd.
+    2: { eapply load_one_of_sep_memlist. 1: eassumption.
+         cbv [dexpr expr expr_body get]. eexists. subst l.
+         rewrite map.get_put_diff; [|congruence].
+         rewrite map.get_put_diff; [|congruence].
+         rewrite map.get_put_same. auto. }
+    (*first store*)
+    cbv [Morphisms.pointwise_relation Basics.impl]. intros. fwd. subst c.
+    rewrite cmd_seq.
+    rewrite <- sep_assoc in H. erewrite idk in H.
+    2: { intros. instantiate (1 := (ptsto b_addr b * ptsto a_addr a)%sep).
+         apply sep_comm. }
+    rewrite sep_assoc in H.
+    eapply WeakestPreconditionProperties.Proper_cmd.
+    2: { eapply store_one_of_sep_memlist. 1: eassumption.
+         - cbv [dexpr expr expr_body get]. eexists. subst l.
+           rewrite map.get_put_diff by congruence.
+           rewrite map.get_put_diff by congruence.
+           rewrite map.get_put_same. auto.
+         - cbv [dexpr expr expr_body get]. eexists. subst l.
+           rewrite map.get_put_same. auto. }
+    (*second store*)
+    cbv [Morphisms.pointwise_relation Basics.impl].
+    intros. fwd.
+    rewrite <- sep_assoc in H0p1.
+    erewrite idk in H0p1.
+    2: { intros. instantiate (1 := (ptsto _ _ * ptsto _ _)%sep). apply sep_comm. }
+    rewrite sep_assoc in H0p1.
+    eapply WeakestPreconditionProperties.Proper_cmd.
+    2: { eapply store_one_of_sep_memlist. 1: eassumption.
+         - cbv [dexpr expr expr_body get]. eexists. subst l.
+           rewrite map.get_put_diff by congruence.
+           rewrite map.get_put_diff by congruence.
+           rewrite map.get_put_diff by congruence.
+           rewrite map.get_put_same. auto.
+         - cbv [dexpr expr expr_body get]. eexists. subst l.
+           rewrite map.get_put_diff by congruence.
+           rewrite map.get_put_same. auto. }
+    (*postcondition*)
+    cbv [Morphisms.pointwise_relation Basics.impl].
+    intros. fwd. cbn [list_map list_map_body]. split; [reflexivity|].
+    split; [|reflexivity]. repeat rewrite byte_to_word_to_byte in H0p2.
+    rewrite <- sep_assoc in H0p2. apply H0p2.
+  Qed.
 
-  Lemma link_swap_swap_swap_swap : spec_of_swap_swap (map.of_list &[,swap_swap; swap]).
-  Proof. eauto using swap_swap_ok, swap_ok. Qed.
+  Definition stackswap := func! (a, b) ~> (b, a) {
+    stackalloc 4 as x;                          
+    store1(x, a);
+    stackalloc 4 as y;                          
+    store1(y, b);
+    swap(y, x);
+    load1(a, x);
+    load1(b, y)
+  }.
 
-  (* Print Assumptions link_swap_swap_swap_swap. *)
-  (*
-  From bedrock2 Require Import ToCString PrintString.
-  Goal True. print_string (c_module &[,swap_swap; swap]). Abort.
-  *)
+  Check byte_to_word_to_byte.
+  Instance spec_of_stackswap : spec_of "stackswap" :=
+    fnspec! "stackswap" a b / abyte bbyte ~> B A,
+    { requires t m := a = of_bytes [abyte] /\ b = of_bytes [bbyte];
+      ensures t' m' := t' = t /\ m' = m /\ A = b /\ B = a }.
+
+  Check load_one_of_sep_memlist.
+  
+  Lemma cmd_stackalloc e x n s t m l post :
+    cmd e (cmd.stackalloc x n s) t m l post = (n mod bytes_per_word 32 = 0 /\
+   (forall (a : word) (mStack mCombined : listmem),
+    anybytes' a (BinIntDef.Z.to_nat n) mStack ->
+    map.split mCombined m mStack ->
+    dlet.dlet (map.put l x a)
+      (fun l0 : locals =>
+       cmd e s t mCombined l0
+         (fun (t' : trace) (mCombined' : listmem) (l' : locals) =>
+          exists m' mStack' : listmem,
+            anybytes' a (BinIntDef.Z.to_nat n) mStack' /\
+            map.split mCombined' m' mStack' /\ post t' m' l')))).
+  Proof. reflexivity. Qed.
+
+  Check cmd.call.
+  Lemma cmd_call e args f rets t m l post :
+    cmd e (cmd.call args f rets) t m l post = (exists args0 : list word,
+     dexprs l rets args0 /\
+     call e f t m args0
+       (fun (t0 : trace) (m0 : listmem) (rets0 : list word) =>
+        exists l' : locals,
+          map.putmany_of_list_zip args rets0 l = Some l' /\ post t0 m0 l')).
+  Proof. reflexivity. Qed.
+
+  Lemma stackswap_ok : program_logic_goal_for_function! stackswap.
+  Proof.
+    repeat straightline. Fail unfold1_cmd_goal. (*why*)
+    (*first stackalloc*)
+    rewrite cmd_stackalloc. split; [reflexivity|]. intros.
+    replace (BinIntDef.Z.to_nat 4) with 4%nat in H0 by reflexivity.
+    cbv [dlet.dlet]. rewrite cmd_seq.
+    destruct H0 as (bs&Hlenbs&H0).
+    assert (mCombined =* array_byte a0 bs * (eq m)).
+    { eexists. eexists. split. 1: apply map.split_comm. 1: eassumption. eauto. }
+    destruct bs as [|? bs]; [discriminate Hlenbs|]. simpl in H2.
+    rewrite sep_assoc in H2.
+    (*first store*)
+    eapply WeakestPreconditionProperties.Proper_cmd.
+    2: { eapply store_one_of_sep_memlist. 1: eassumption.
+         - cbv [dexpr expr expr_body get]. eexists. subst l.
+           repeat (rewrite map.get_put_diff by congruence).
+           rewrite map.get_put_same. auto.
+         - cbv [dexpr expr expr_body get]. eexists. subst l.
+           repeat (rewrite map.get_put_diff by congruence).
+           rewrite map.get_put_same. auto. }
+    cbv [Morphisms.pointwise_relation Basics.impl]. intros. fwd.
+    subst a. rewrite byte_to_word_to_byte in H3p1.
+    (*second stackalloc*)
+    rewrite cmd_stackalloc. split; [reflexivity|]. intros.
+    replace (BinIntDef.Z.to_nat 4) with 4%nat in H3 by reflexivity.
+    cbv [dlet.dlet]. rewrite cmd_seq.
+    destruct H3 as (bs2&Hlenbs2&H3).
+    assert (mCombined0 =* array_byte a bs2 * (ptsto a0 abyte ⋆ (array_byte (word.add a0 (word.of_Z 1)) bs ⋆ eq m))).
+    { eexists. eexists. split. 1: apply map.split_comm. 1: eassumption. eauto. }
+    destruct bs2 as [|? bs2]; [discriminate Hlenbs2|]. simpl in H5.
+    rewrite sep_assoc in H5.
+    (*second store*)
+    eapply WeakestPreconditionProperties.Proper_cmd.
+    2: { eapply store_one_of_sep_memlist. 1: eassumption.
+         - cbv [dexpr expr expr_body get]. eexists. subst l.
+           repeat (rewrite map.get_put_diff by congruence).
+           rewrite map.get_put_same. auto.
+         - cbv [dexpr expr expr_body get]. eexists. subst l.
+           repeat (rewrite map.get_put_diff by congruence).
+           rewrite map.get_put_same. auto. }
+    cbv [Morphisms.pointwise_relation Basics.impl]. intros. fwd.
+    subst b. rewrite byte_to_word_to_byte in H6p1.
+    (*function call*)
+    rewrite cmd_seq. rewrite cmd_call. eexists. split.
+    { cbv [dexprs list_map list_map_body expr expr_body get]. eexists. split.
+      - rewrite map.get_put_same. reflexivity.
+      - eexists. split.
+        + rewrite map.get_put_diff by congruence. rewrite map.get_put_same. reflexivity.
+        + reflexivity. }
+    clear H5. clear H2. clear H3p1. rewrite <- sep_assoc in H6p1.
+    rewrite <- sep_assoc in H6p1. erewrite idk in H6p1.
+    2: { intros. instantiate (1 := (ptsto _ _ * ptsto _ _ * _)%sep).
+         erewrite idk.
+         2: { intros. instantiate (1 := (_ * ptsto _ _)%sep). apply sep_comm. }
+         rewrite sep_assoc. rewrite sep_comm. reflexivity. }
+    rewrite sep_assoc in H6p1.
+    straightline_call. 1: eassumption. fwd. eexists. split; [reflexivity|].
+    (*first load*)
+    rewrite cmd_seq. clear H6p1.
+    erewrite idk in H2p1.
+    2: { intros. instantiate (1 := (ptsto _ _ * ptsto _ _)%sep). apply sep_comm. }
+    rewrite sep_assoc in H2p1.
+    eapply WeakestPreconditionProperties.Proper_cmd.
+    2: { eapply load_one_of_sep_memlist. 1: eassumption.
+         - cbv [dexpr expr expr_body get]. eexists. subst l.
+           repeat (rewrite map.get_put_diff by congruence).
+           rewrite map.get_put_same. auto. }
+    cbv [Morphisms.pointwise_relation Basics.impl]. intros. fwd.
+    (*second load*)
+    rewrite <- sep_assoc in H2p1.
+    erewrite idk in H2p1.
+    2: { intros. instantiate (1 := (ptsto _ _ * ptsto _ _)%sep). apply sep_comm. }
+    rewrite sep_assoc in H2p1.
+    eapply WeakestPreconditionProperties.Proper_cmd.
+    2: { eapply load_one_of_sep_memlist. 1: eassumption.
+         - cbv [dexpr expr expr_body get]. eexists. subst l.
+           repeat (rewrite map.get_put_diff by congruence).
+           rewrite map.get_put_same. auto. }
+    cbv [Morphisms.pointwise_relation Basics.impl]. intros. fwd.
+    (*first stackdealloc*)
+    do 2 rewrite <- sep_assoc in H2p1. erewrite idk in H2p1.
+    2: { intros. instantiate (1 := (array_byte _ _ * ptsto _ _)%sep). rewrite sep_assoc.
+         rewrite sep_comm. erewrite idk.
+         2: { intros. instantiate (1 := (_ * ptsto _ _)%sep). apply sep_comm. }
+         rewrite sep_comm. rewrite <- sep_assoc. instantiate (3 := (abyte :: bs2)).
+         simpl. reflexivity. }
+    rewrite sep_assoc in H2p1.
+    destruct H2p1 as (mStack' & m' & Hsplit & HmStack' & Hm').
+    exists m', mStack'. split.
+    { eexists. split; [|eassumption]. simpl in Hlenbs2. simpl. lia. }
+    split.
+    { apply map.split_comm. assumption. }
+    (*second stackdealloc*)
+    rewrite <- sep_assoc in Hm'.
+    eassert (array_byte a0 (bbyte :: bs) = _) as arr.
+    { simpl. reflexivity. }
+    rewrite <- arr in Hm'. clear arr.
+    destruct Hm' as (mStack'0 & m'0 & Hsplit0 & HmStack'0 & Hm'0).
+    exists m'0, mStack'0. split.
+    { eexists. split; [|eassumption]. simpl in Hlenbs. simpl. lia. }
+    split.
+    { apply map.split_comm. assumption. }
+    (*postcondition*)
+    cbv [list_map list_map_body get]. eexists. split.
+    { repeat (rewrite map.get_put_diff by congruence). rewrite map.get_put_same. auto. }
+    eexists. split.
+    { repeat (rewrite map.get_put_diff by congruence). rewrite map.get_put_same. auto. }
+    eexists. eexists. eauto.
+  Qed.
+  Print Assumptions stackswap_ok.
+
+(*
+Section Variables:
+    word_ok : word.ok word
+    word : Interface.word 32
+    mem_ok : map.ok mem
+    mem : map.map word (Init.Byte.byte : Type)
+    locals_ok : map.ok locals
+    locals : map.map String.string word
+    listmem_ok : map.ok listmem
+    listmem : map.map (word * nat) (Init.Byte.byte : Type)
+    ext_spec_ok : ext_spec.ok ext_spec
+    ext_spec : ExtSpec
+    BW : Bitwidth 32
+
+Axioms:
+    wordnat_eqb_spec :
+        forall (width : Z) (BW : Bitwidth width) (word : Interface.word width)
+        (listmem : map.map (word * nat) (Init.Byte.byte : Type)),
+        word.ok word -> EqDecider wordnat_eqb
+    wordnat_eqb :
+        forall width : Z,
+        Bitwidth width ->
+        forall word : Interface.word width,
+        map.map (word * nat) (Init.Byte.byte : Type) -> word * nat -> word * nat -> bool
+*)
 End WithParameters.
